examples/mw/MWHeader.v
@@ -42,6 +42,7 @@ Program Instance t: URA.t := {
   unit := unit;
   _add := add;
   _wf := wf;
+  core := fun _ => unit;
 }
 .
 Next Obligation. subst add wf. i. destruct a, b; ss; des_ifs; ss. Qed.
@@ -49,6 +50,11 @@ Next Obligation. subst add wf. i. destruct a, b; ss; des_ifs; ss. Qed.
 Next Obligation. subst add wf. i. unseal "ra". des_ifs. Qed.
 Next Obligation. subst add wf. i. unseal "ra". ss. Qed.
 Next Obligation. subst add wf. i. unseal "ra". des_ifs. Qed.
+Next Obligation. subst add wf. i. unseal "ra". des_ifs. Qed.
+Next Obligation. subst add wf. i. unseal "ra". des_ifs. Qed.
+Next Obligation.
+  i. exists unit. subst add. unseal "ra". des_ifs.
+Qed.
 
 End AppRA.
 End AppRA.
@@ -352,7 +358,7 @@ Definition set `{Dec K} V (k: K) (v: V) (f: K -> V): K -> V := fun k0 => if dec 
 
 Section PROOF.
   Context `{Σ: GRA.t}.
-  
+
   Lemma Own_unit
     :
       bi_entails True%I (Own ε)
